Some shuffle of code

src/Frontend/Approval.v
@@ -45,15 +45,16 @@ Section Approval.
       c : challenge -- I need to think about making it non-interactive (fiat-shamir)
    *)
 
-   (* In this function, when you pass a value of m that not 0 and 1, the 
-    function still creates a proof but it won't pass the check 
-    of verify_encryption_vote_proof, which checks if cp is encryption of 
-    zero or one. See the proofs vote_proof_valid and vote_proof_invalid *)
-    Definition encrypt_vote_and_generate_enc_proof 
+   
+
+    (* encrypt vote *)
+    Definition encrypt_vote (r : F) (g h : G) (m : F) : G * G :=
+      @enc F G gop gpow g h m r.
+
+    (* create a proof *)
+    Definition generate_enc_proof 
       (r : F) (g h : G) (m : F) 
-      (uscs : Vector.t F 3) (c : F) : G * G * @Sigma.sigma_proto F (G * G) 2 3 2 := 
-      let cp := @enc F G gop gpow g h m r in
-      let sig_proof := 
+      (uscs : Vector.t F 3) (cp : G * G) (c : F) : @Sigma.sigma_proto F (G * G) 2 3 2 :=
         match Fdec m zero with 
         | left _ => 
           @generalised_construct_encryption_proof_elgamal_real F zero add mul sub 
@@ -63,7 +64,19 @@ Section Approval.
           @generalised_construct_encryption_proof_elgamal_real F zero add mul sub 
             opp G ginv gop gpow 0 (Fin.FS Fin.F1) r uscs [g^zero; g^m] g h cp c (* real one 
             goes to the second place (Fin.FS Fin.F1) *)
-        end 
+        end.
+
+    
+    (* wrap both of them *)
+    (* In this function, when you pass a value of m that not 0 and 1, the 
+    function still creates a proof but it won't pass the check 
+    of verify_encryption_vote_proof, which checks if cp is encryption of 
+    zero or one. See the proofs vote_proof_valid and vote_proof_invalid *)
+    Definition encrypt_vote_and_generate_enc_proof 
+      (r : F) (g h : G) (m : F) 
+      (uscs : Vector.t F 3) (c : F) : G * G * @Sigma.sigma_proto F (G * G) 2 3 2 := 
+      let cp := @enc F G gop gpow g h m r in
+      let sig_proof := generate_enc_proof r g h m uscs cp c
       in (cp, sig_proof).
 
     (* verification of encryption proof *)
@@ -75,7 +88,43 @@ Section Approval.
       end.
 
 
-    (* encrypts the whole ballot. *)
+    (* encrypt the whole ballot *)
+    Fixpoint encrypt_ballot {n : nat}
+      (r : Vector.t F n) (g h : G) (m : Vector.t F n) : Vector.t (G * G) n.
+    Proof.
+       destruct n as [| n].
+      +
+        exact [].
+      +
+        destruct (vector_inv_S r) as (rh & rt & _).
+        destruct (vector_inv_S m) as (mh & mt & _).
+        exact (encrypt_vote rh g h mh :: encrypt_ballot _ rt g h mt).
+    Defined.
+
+    (* generate enc proof for a ballot *)
+    Fixpoint generate_enc_proof_ballot {n : nat}
+      (r : Vector.t F n) (g h : G) (m : Vector.t F n) 
+      (uscs : Vector.t (Vector.t F 3) n) 
+      (cp : Vector.t (G * G) n) (c : Vector.t F n) : 
+      Vector.t (@Sigma.sigma_proto F (G * G) 2 3 2) n.
+    Proof.
+       destruct n as [| n].
+      +
+        exact [].
+      +
+        destruct (vector_inv_S r) as (rh & rt & _).
+        destruct (vector_inv_S m) as (mh & mt & _).
+        destruct (vector_inv_S uscs) as (uscsh & uscst & _).
+        destruct (vector_inv_S cp) as (cph & cpt & _).
+        destruct (vector_inv_S c) as (ch & ct & _).
+        exact(generate_enc_proof rh g h mh uscsh cph ch :: 
+          generate_enc_proof_ballot _ rt g h mt uscst cpt ct).
+    Defined.
+
+
+
+
+    (* encrypts the whole ballot and generate proof *)
     Fixpoint encrypt_ballot_and_generate_enc_proof {n : nat}
       (r : Vector.t F n) (g h : G) (m : Vector.t F n) 
       (uscs : Vector.t (Vector.t F 3) n) (c : Vector.t F n) : 
@@ -95,9 +144,8 @@ Section Approval.
     Defined.
 
 
-    
     Fixpoint verify_encryption_ballot_proof {n : nat} (g h : G)
-    (cppf : Vector.t (G * G * @Sigma.sigma_proto F (G * G) 2 3 2) n) : bool.
+      (cppf : Vector.t (G * G * @Sigma.sigma_proto F (G * G) 2 3 2) n) : bool.
     Proof.
       destruct n as [| n].
       +
@@ -109,415 +157,497 @@ Section Approval.
     Defined.
 
 
-  End Definitions.
+    End Definitions.
 
-  Section Proofs.
-
-    (* Vector Space *)
-      Context
-        {Hvec: @vector_space F (@eq F) zero one add mul sub 
-        div opp inv G (@eq G) gid ginv gop gpow}.
-
-      
-      (* add field *)
-      Add Field field : (@field_theory_for_stdlib_tactic F
-        eq zero one opp add mul sub inv div vector_space_field).
-
+    Section Proofs.
     
-    Theorem encryption_correct : ∀ (r : F) (g h : G) (m : F) 
-      (uscs : Vector.t F 3) (c : F),
-      let (cp, _) := encrypt_vote_and_generate_enc_proof r g h m uscs c in
-      cp = @enc F G gop gpow g h m r.
-    Proof.
-      intros *. 
-      unfold encrypt_vote_and_generate_enc_proof, enc.
-      destruct (Fdec m zero).
-      - (* Case m = zero *) 
-        reflexivity.  (* Directly reduces to (gʳ, hʳ) *)
-      - (* Case m = one *)
-        reflexivity.  (* Directly reduces to (gʳ, g¹·hʳ) *)
-    Qed.
+      (* Vector Space *)
+        Context
+          {Hvec: @vector_space F (@eq F) zero one add mul sub 
+          div opp inv G (@eq G) gid ginv gop gpow}.
 
-    Theorem vote_proof_valid :
-      ∀ (r : F) (g h : G) (m : F) (uscs : Vector.t F 3) (c : F),
-        (m = zero ∨ m = one) →
-        verify_encryption_vote_proof g h 
-          (encrypt_vote_and_generate_enc_proof r g h m uscs c) = true.
-    Proof.
-      intros * ha.
-      unfold encrypt_vote_and_generate_enc_proof, 
-      verify_encryption_vote_proof.
-      destruct (Fdec m zero) as [fa | fa].
-      +
-        subst.
-        eapply generalised_construct_encryption_proof_elgamal_real_completeness.
-        (* I had a mini-heart attack by looking at the goal :) *)
-        subst; cbn. split. reflexivity.
-        assert (Hwt : gop (g ^ zero) (h ^ r) = gop (h ^ r) (g ^ zero)).
-        rewrite commutative; reflexivity.
-        rewrite Hwt; clear Hwt.
-        setoid_rewrite <-(@monoid_is_associative G (@eq G) gop gid).
-        assert (Hwt : (gop (g ^ zero) (gop (ginv (g ^ zero)) (h ^ r))) = 
-        (h ^ r)).
-        rewrite associative.
-        rewrite group_is_right_inverse,
-        monoid_is_left_idenity;
-        reflexivity. rewrite associative, commutative in Hwt.
-        rewrite Hwt. reflexivity. 
-        typeclasses eauto.
-      +
-        destruct ha as [ha | ha]; try congruence. subst.
-        eapply generalised_construct_encryption_proof_elgamal_real_completeness.
-         (* m = 1 *)
-        split. reflexivity.
-        cbn. subst.
-        assert (Hwt : gop (g ^ one) (h ^ r) = gop (h ^ r) (g ^ one)).
-        rewrite commutative; reflexivity.
-        rewrite Hwt; clear Hwt.
-        setoid_rewrite <-(@monoid_is_associative G (@eq G) gop gid).
-        assert (Hwt : (gop (g ^ one) (gop (ginv (g ^ one)) (h ^ r))) = 
-        (h ^ r)).
-        rewrite associative.
-        rewrite group_is_right_inverse,
-        monoid_is_left_idenity;
-        reflexivity. rewrite associative, commutative in Hwt.
-        rewrite Hwt. reflexivity. 
-        typeclasses eauto.
-    Qed.
-
-
-    Lemma mul_eq_zero (a b : F) : a * b = zero → a = zero ∨ b = zero.
-    Proof.
-      intro ha.  (* Assume a * b = 0 *)
-      (* Case analysis on whether a = 0 *)
-      destruct (Fdec a zero) as [hb | hb].
-      - (* Case 1: a = 0 *)
-        left; assumption.
-      - (* Case 2: a ≠ 0 *)
-        right.
-        eapply f_equal with (f := fun x => inv a * x) in ha.
-        rewrite associative in ha.
-        assert (hc : inv a * a = one). field.
-        assumption.
-        rewrite hc in ha; clear hc.
-        assert (hc : inv a * zero = zero). field.
-        assumption. rewrite hc in ha; clear hc.
-        assert (hc : one * b = b). field.
-        rewrite hc in ha. exact ha.
-    Qed.
-
-    Lemma sub_eq : forall (u v : F), sub u v = zero -> u = v.
-    Proof.
-      intros * ha.
-      assert (hb : sub u v = u + opp v). field.
-      rewrite hb in ha.
-      eapply f_equal with (f := fun x => x + v) in ha.
-      assert (hc : opp v + v = zero). field.
-      rewrite <-associative in ha.
-      rewrite hc in ha; clear hc.
-      assert (hc : u + zero = u) by field.
-      rewrite hc in ha; clear hc.
-      assert (hc : zero + v = v) by field.
-      rewrite hc in ha. exact ha.
-    Qed.
-      
-    
-    Theorem vote_proof_invalid_reject :
-      ∀ (r : F) (g h : G) (m : F)  (u₁ u₂ c₁ : F) (c : F),
-        g <> gid -> (m <> zero ∧ m <> one) → c₁ <> c ->
-        verify_encryption_vote_proof g h 
-          (encrypt_vote_and_generate_enc_proof r g h m [u₁; u₂; c₁] c) = false.
-    Proof.
-      intros * ht hu hv.
-      unfold encrypt_vote_and_generate_enc_proof, 
-      verify_encryption_vote_proof.
-      destruct (Fdec m zero) as [fa | fa].
-      +
         
-        destruct hu as (hal & har).
-        subst. specialize (hal eq_refl).
-        inversion hal.
-      +
-        destruct (Fdec m one) as [faa | faa].
-        ++
-          subst; destruct hu as (hal & har).
-          specialize (har eq_refl). 
-          inversion har.
-        ++
-          (* challenging case *)
-          unfold generalised_accepting_encryption_proof_elgamal, 
-          enc, generalised_construct_encryption_proof_elgamal_real.
-          simpl. 
-          destruct (vector_fin_app_pred 1 (FS F1) [u₁; u₂] [c₁]) as
-          (m₁ & m₂ & v₁ & v₃ & vm & v₂ & v₄ & pfaa & pfbb & haa).
-          destruct pfaa as [pfa].
-          destruct pfbb as [pfb].
-          destruct haa as [ha].
-          destruct ha as (ha & hb & hc & hd).
-          subst; cbn in * |- *.
-          assert (m₂ = 0). 
-          {
-            destruct m₂ as [|m₂].
-            reflexivity. nia.
-          }
+        (* add field *)
+        Add Field field : (@field_theory_for_stdlib_tactic F
+          eq zero one opp add mul sub inv div vector_space_field).
+
+      Theorem first_projection_vote_encryption : 
+        ∀ (r : F) (g h : G) (m : F) 
+        (uscs : Vector.t F 3) (c : F), 
+        fst (encrypt_vote_and_generate_enc_proof r g h m uscs c) = 
+        encrypt_vote r g h m.
+      Proof.
+        intros *; 
+        unfold encrypt_vote_and_generate_enc_proof, 
+        enc, encrypt_vote, enc; cbn.
+        reflexivity.
+      Qed.
+
+      Theorem second_projection_vote_sigma_proof : 
+        ∀ (r : F) (g h : G) (m : F) 
+        (uscs : Vector.t F 3) (cp : G * G) (c : F), 
+        cp =  @enc F G gop gpow g h m r  -> 
+        snd (encrypt_vote_and_generate_enc_proof r g h m uscs c) = 
+        generate_enc_proof r g h m uscs cp c.
+      Proof.
+        intros * ha.
+        unfold encrypt_vote_and_generate_enc_proof, 
+        generate_enc_proof; subst.  simpl.
+        reflexivity.
+      Qed.
+
+
+      Theorem first_project_ballot_encryption : 
+        ∀ (n : nat) (r : Vector.t F n) (g h : G) (m : Vector.t F n) 
+          (uscs : Vector.t (Vector.t F 3) n) (c : Vector.t F n),
+        Vector.map fst (encrypt_ballot_and_generate_enc_proof r g h m uscs c) = 
+        encrypt_ballot r g h m.
+      Proof.
+        induction n as [|n ihn].
+        +
+          intros *. 
+          reflexivity.
+        +
+          intros *.
+          destruct (vector_inv_S r) as (rh & rt & ha).
+          destruct (vector_inv_S m) as (mh & mt & hb).
+          destruct (vector_inv_S uscs) as (uscsh & uscst & hc).
+          destruct (vector_inv_S c) as (ch & ct & hd).
           subst. cbn. 
-          assert (pfa = eq_refl). 
-          eapply Eqdep_dec.UIP_refl_nat.
-          assert (pfb = eq_refl). 
-          eapply Eqdep_dec.UIP_refl_nat.
-          subst. cbn in * |- *.
-          pose proof (vector_inv_0 v₂) as hd.
-          pose proof (vector_inv_0 v₄) as he.
-          rewrite hd, he in * |- *. cbn.
-          subst; cbn.
-          destruct (vector_inv_S v₁) as (ma & msr & hmm).
-          rewrite hmm in * |- *.
-          subst; cbn.
-          pose proof (vector_inv_0 msr) as hd.
-          subst; cbn.
-          destruct (vector_inv_S v₃) as (mb & msr & hmm).
-          subst; cbn.
-          pose proof (vector_inv_0 msr) as hd.
-          subst; cbn.
-          assert (hd : c = (c₁ + (sub c (c₁ + zero) + zero))). field.
-          rewrite <-hd; clear hd.
-          destruct (Fdec c c)
-          as [hdec | hdec]; try auto. 
-          eapply Bool.andb_false_intro2.
-          eapply Bool.andb_false_intro1.
-          eapply Bool.andb_false_intro2.
-          eapply dec_false; intro haa.
-          assert (hb : c₁ + zero = c₁). field.
-          rewrite !hb in haa; clear hb.
-          assert(hb : g ^ one = g).
-          rewrite field_one; reflexivity.
-          rewrite !hb in haa; clear hb.
-          assert (hb : gop (g ^ m) (h ^ r) = gop (h ^ r) (g ^ m)).
-          rewrite commutative. reflexivity.
-          rewrite !hb in haa; clear hb.
-          assert (hb : (gop (gop (h ^ r) (g ^ m)) (ginv g)) = 
-           gop (h ^ r) (gop (g ^ m) (ginv g))).
-          rewrite associative; reflexivity.
-          rewrite !hb in haa; clear hb.
-          remember ((gop (g ^ m) (ginv g))) as gp.
-          rewrite smul_distributive_vadd, smul_pow_mul,
-          associative in haa.
-          assert (hb : (gop (h ^ u₂) (h ^ (sub c c₁ * r))) = 
-            h ^ (u₂ + sub c c₁ * r)).
-          destruct Hvec. (* why do I need this destruct this? *)
-          setoid_rewrite <-vector_space_smul_distributive_fadd;
+          rewrite ihn.
+          unfold encrypt_vote.
           reflexivity.
-          rewrite hb in haa; clear hb.
-          eapply f_equal with (f := fun x => 
-            gop (h ^ (opp (u₂ + sub c c₁ * r))) x) in haa.
-          assert (hb : gop (h ^ opp (u₂ + sub c c₁ * r)) (h ^ (u₂ + sub c c₁ * r)) = gid).
-          destruct Hvec.
-          setoid_rewrite <-vector_space_smul_distributive_fadd.
-          assert (hb : (opp (u₂ + sub c c₁ * r) + (u₂ + sub c c₁ * r)) = zero). field.
-          rewrite hb; clear hb.
-          rewrite field_zero; reflexivity.
-          rewrite !hb in haa; clear hb.
-          rewrite associative in haa.
-          assert (hb : gop (h ^ opp (u₂ + sub c c₁ * r)) (h ^ (u₂ + sub c c₁ * r)) = 
-           gid). destruct Hvec.
-          rewrite <-vector_space_smul_distributive_fadd.
-          assert (hb : (opp (u₂ + sub c c₁ * r) + (u₂ + sub c c₁ * r)) = zero).
-          field. rewrite hb; clear hb.
-          rewrite field_zero; reflexivity.
-          rewrite hb in haa; clear hb.
-          rewrite left_identity in haa.
-          rewrite Heqgp in haa; clear Heqgp.
-          rewrite <- (vector_space_field_zero g) in haa.
-          assert (hb : gop (g ^ m) (ginv g) ^ sub c c₁ = 
-            gop ((g ^ m) ^ sub c c₁) (ginv g ^ sub c c₁)).
-          destruct Hvec.
-          rewrite vector_space_smul_distributive_vadd; reflexivity.
-          rewrite hb in haa; clear hb.
-          eapply f_equal with (f := fun x => gop x (g ^ sub c c₁)) in haa.
-          rewrite <-associative in haa.
-          assert (hb : (gop (ginv g ^ sub c c₁) (g ^ sub c c₁)) = gid).
-          destruct Hvec.
-          rewrite <-vector_space_smul_distributive_vadd, left_inverse, 
-          <-field_zero, smul_pow_up.
-          assert (hb : zero * sub c c₁ = zero). field.
-          rewrite hb; clear hb.
+      Qed.
+
+
+
+      Theorem second_project_ballot_sigma_proof : 
+        ∀ (n : nat) (r : Vector.t F n) (g h : G) (m : Vector.t F n) 
+        (uscs : Vector.t (Vector.t F 3) n) (cp : Vector.t (G * G) n) (c : Vector.t F n),
+        (∀ (i : Fin.t n), Vector.nth cp i = @enc F G gop gpow g h (Vector.nth m i) (Vector.nth r i)) ->
+        Vector.map snd (encrypt_ballot_and_generate_enc_proof r g h m uscs c) = 
+        generate_enc_proof_ballot r g h m uscs cp c.
+      Proof.  
+        induction n as [|n ihn].
+        +
+          intros * ha.
           reflexivity.
-          rewrite hb in haa; clear hb.
-          destruct Hvec.
-          rewrite <- vector_space_smul_distributive_fadd, right_identity,
-          smul_pow_up in haa.
-          assert (hb : zero + sub c c₁ = sub c c₁). field.
-          rewrite hb in haa; clear hb.
-          eapply f_equal with (f := fun x => gop x (g ^ opp (sub c c₁))) in haa.
-          assert(hb : gop (g ^ sub c c₁) (g ^ opp (sub c c₁)) = gid).
-          destruct Hvec.
-          rewrite <-vector_space_smul_distributive_fadd.
-          assert(hb : (sub c c₁ + opp (sub c c₁)) = zero). field.
-          rewrite hb; clear hb.
-          rewrite field_zero; reflexivity.
-          rewrite !hb in haa; clear hb.
-          rewrite  <-smul_distributive_fadd in haa.
-          assert (hb : (m * sub c c₁ + opp (sub c c₁)) = 
-            (sub m one) * sub c c₁). field.
-          rewrite hb in haa; clear hb.
-          eapply eq_sym in haa.
-          eapply gid_power_zero in haa.
-          destruct haa as [haa | haa]; try congruence.
-          eapply mul_eq_zero in haa.
-          destruct haa as [haa | haa].
-          +++
-            eapply faa.
-            eapply sub_eq;
-            assumption.
-          +++
-            eapply hv.
-            eapply eq_sym.
-            eapply sub_eq.
-            assumption.
-        Unshelve.
-        exact g. exact Fdec.
-    Qed.
+        +
+          intros * hf.
+          destruct (vector_inv_S r) as (rh & rt & ha).
+          destruct (vector_inv_S m) as (mh & mt & hb).
+          destruct (vector_inv_S uscs) as (uscsh & uscst & hc).
+          destruct (vector_inv_S cp) as (cph & cpt & hd).
+          destruct (vector_inv_S c) as (ch & ct & he).
+          subst. cbn. f_equal.
+          specialize (hf Fin.F1); cbn in hf.
+          subst. reflexivity.
+          eapply ihn. intro f.
+          specialize (hf (Fin.FS f)).
+          cbn in hf. exact hf.
+      Qed.
+          
 
 
-    (* 
-      A theorem that states that if the prover can predict the challenge of 
-      the verifier, then it can fake the proof. 
 
+      
+      Theorem encryption_correct : ∀ (r : F) (g h : G) (m : F) 
+        (uscs : Vector.t F 3) (c : F),
+        match encrypt_vote_and_generate_enc_proof r g h m uscs c with 
+        | (cp, _) => cp = (gpow g r, gop (gpow g m) (gpow h r))
+        end.
+      Proof.
+        intros *. 
+        unfold encrypt_vote_and_generate_enc_proof, enc.
+        destruct (Fdec m zero).
+        - (* Case m = zero *) 
+          reflexivity.  (* Directly reduces to (gʳ, hʳ) *)
+        - (* Case m = one *)
+          reflexivity.  (* Directly reduces to (gʳ, g¹·hʳ) *)
+      Qed.
 
-      if it is the case c = c₁ then 
-      an invalid proof will also be accepted but 
-      c = c₁ will happen with 1/|C| probability.
-    *)
-    Theorem vote_proof_invalid_accept :
-      ∀ (r : F) (g h : G) (m : F)  (u₁ u₂ c₁ : F) (c : F),
-        (m <> zero ∧ m <> one) → c₁ = c ->
-        verify_encryption_vote_proof g h 
-          (encrypt_vote_and_generate_enc_proof r g h m [u₁; u₂; c₁] c) = true.
-    Proof.
-      intros * [hal har] hb.
-       unfold encrypt_vote_and_generate_enc_proof, 
-      verify_encryption_vote_proof.
-      eapply generalised_accepting_elgamal_conversations_correctness_gen.
-      destruct (Fdec m zero) as [fa | fa]; try congruence.
-      subst.
-      unfold generalised_accepting_encryption_proof_elgamal, 
-      enc, generalised_construct_encryption_proof_elgamal_real.
-      simpl. 
-      destruct (vector_fin_app_pred 1 (FS F1) [u₁; u₂] [c]) as
-        (m₁ & m₂ & v₁ & v₃ & vm & v₂ & v₄ & pfaa & pfbb & haa).
-      destruct pfaa as [pfa].
-      destruct pfbb as [pfb].
-      destruct haa as [ha].
-      destruct ha as (ha & hb & hc & hd).
-      subst; cbn in * |- *.
-      assert (m₂ = 0). 
-      {
-        destruct m₂ as [|m₂].
-        reflexivity. nia.
-      }
-      subst. cbn. 
-      assert (pfa = eq_refl). 
-      eapply Eqdep_dec.UIP_refl_nat.
-      assert (pfb = eq_refl). 
-      eapply Eqdep_dec.UIP_refl_nat.
-      subst. cbn in * |- *.
-      pose proof (vector_inv_0 v₂) as hd.
-      pose proof (vector_inv_0 v₄) as he.
-      rewrite hd, he in * |- *. cbn.
-      subst; cbn.
-      destruct (vector_inv_S v₁) as (ma & msr & hmm).
-      rewrite hmm in * |- *.
-      subst; cbn.
-      pose proof (vector_inv_0 msr) as hd.
-      subst; cbn.
-      destruct (vector_inv_S v₃) as (mb & msr & hmm).
-      subst; cbn.
-      pose proof (vector_inv_0 msr) as hd.
-      subst; cbn.
-      assert (hd : c = (c + (sub c (c + zero) + zero))). field.
-      rewrite <-hd; clear hd.
-      split. reflexivity.
-      intros f. rewrite !dec_true.
-      destruct (fin_inv_S _ f) as [f' | (f' & hf)].
-      +
-        subst; cbn.
-        split.
-        ++
-          pose proof @simulator_completeness F zero one add mul sub div opp inv 
-            G gid ginv gop gpow Gdec Hvec g (g ^ r) u₁ c as hb.
-          unfold accepting_conversation, schnorr_simulator in hb.
-          rewrite dec_true in hb; cbn in hb.
-          exact hb.
-        ++
-          assert(hb :  (ginv (g ^ zero)) = gid). 
-          rewrite field_zero, group_inv_id;
-          reflexivity.
-          rewrite !hb; clear hb.
-          remember (gop (g ^ m) (h ^ r)) as gm.
-          rewrite <-associative.
-          assert (hb : gop (gop gm gid ^ opp c) (gop gm gid ^ c) = gid). 
-          destruct Hvec.
-          rewrite <-vector_space_smul_distributive_fadd.
-          assert (hb : (opp c + c) = zero).
-          field. rewrite hb; clear hb.
-          rewrite field_zero; reflexivity.
-          rewrite hb; clear hb.
-          rewrite right_identity. 
-          reflexivity.
-      +
-        subst; cbn.
-        destruct (fin_inv_S _ f') as [f'' | (f'' & hf)];
-        subst; cbn; (try refine match f'' with end).
-        split.
-        ++
-          assert (hb : sub c (c + zero) * r = zero). field.
-          rewrite !hb; clear hb.
-          assert(hb : sub c (c + zero) = zero). field.
-          rewrite hb; clear hb.
-          rewrite field_zero, right_identity.
-          rewrite right_identity; reflexivity.
-        ++
-          assert (hb : sub c (c + zero) * r = zero). field.
-          rewrite !hb; clear hb.
-          assert(hb : sub c (c + zero) = zero). field.
-          rewrite hb; clear hb.
-          rewrite field_one, field_zero, 
-          right_identity, right_identity.
-          reflexivity.
-    Qed.
-
-
-    (* ballot proof is valid *)
-    Theorem ballot_proof_valid :
-      ∀ (n : nat) (rs : Vector.t F n) (g h : G) 
-        (ms : Vector.t F n) (uscs : Vector.t (Vector.t F 3) n) (chs : Vector.t F n),
-        (∀ (i : Fin.t n), Vector.nth ms i = zero ∨ Vector.nth ms i = one) ->
-        verify_encryption_ballot_proof g h 
-          (encrypt_ballot_and_generate_enc_proof rs g h ms uscs chs) = true.
-    Proof.
-      induction n as [|n ihn].
-      +
+      Theorem vote_proof_valid :
+        ∀ (r : F) (g h : G) (m : F) (uscs : Vector.t F 3) (c : F),
+          (m = zero ∨ m = one) →
+          verify_encryption_vote_proof g h 
+            (encrypt_vote_and_generate_enc_proof r g h m uscs c) = true.
+      Proof.
         intros * ha.
-        pose proof (vector_inv_0 rs) as hb.
-        pose proof (vector_inv_0 ms) as hc.
-        pose proof (vector_inv_0 uscs) as hd.
-        pose proof (vector_inv_0 chs) as he.
-        subst; cbn. reflexivity.
-      +
+        unfold encrypt_vote_and_generate_enc_proof, 
+        verify_encryption_vote_proof, generate_enc_proof.
+        destruct (Fdec m zero) as [fa | fa].
+        +
+          subst.
+          eapply generalised_construct_encryption_proof_elgamal_real_completeness.
+          (* I had a mini-heart attack by looking at the goal :) *)
+          subst; cbn. split. reflexivity.
+          assert (Hwt : gop (g ^ zero) (h ^ r) = gop (h ^ r) (g ^ zero)).
+          rewrite commutative; reflexivity.
+          rewrite Hwt; clear Hwt.
+          setoid_rewrite <-(@monoid_is_associative G (@eq G) gop gid).
+          assert (Hwt : (gop (g ^ zero) (gop (ginv (g ^ zero)) (h ^ r))) = 
+          (h ^ r)).
+          rewrite associative.
+          rewrite group_is_right_inverse,
+          monoid_is_left_idenity;
+          reflexivity. rewrite associative, commutative in Hwt.
+          rewrite Hwt. reflexivity. 
+          typeclasses eauto.
+        +
+          destruct ha as [ha | ha]; try congruence. subst.
+          eapply generalised_construct_encryption_proof_elgamal_real_completeness.
+          (* m = 1 *)
+          split. reflexivity.
+          cbn. subst.
+          assert (Hwt : gop (g ^ one) (h ^ r) = gop (h ^ r) (g ^ one)).
+          rewrite commutative; reflexivity.
+          rewrite Hwt; clear Hwt.
+          setoid_rewrite <-(@monoid_is_associative G (@eq G) gop gid).
+          assert (Hwt : (gop (g ^ one) (gop (ginv (g ^ one)) (h ^ r))) = 
+          (h ^ r)).
+          rewrite associative.
+          rewrite group_is_right_inverse,
+          monoid_is_left_idenity;
+          reflexivity. rewrite associative, commutative in Hwt.
+          rewrite Hwt. reflexivity. 
+          typeclasses eauto.
+      Qed.
+
+
+      Lemma mul_eq_zero (a b : F) : a * b = zero → a = zero ∨ b = zero.
+      Proof.
+        intro ha.  (* Assume a * b = 0 *)
+        (* Case analysis on whether a = 0 *)
+        destruct (Fdec a zero) as [hb | hb].
+        - (* Case 1: a = 0 *)
+          left; assumption.
+        - (* Case 2: a ≠ 0 *)
+          right.
+          eapply f_equal with (f := fun x => inv a * x) in ha.
+          rewrite associative in ha.
+          assert (hc : inv a * a = one). field.
+          assumption.
+          rewrite hc in ha; clear hc.
+          assert (hc : inv a * zero = zero). field.
+          assumption. rewrite hc in ha; clear hc.
+          assert (hc : one * b = b). field.
+          rewrite hc in ha. exact ha.
+      Qed.
+
+      Lemma sub_eq : forall (u v : F), sub u v = zero -> u = v.
+      Proof.
         intros * ha.
-        destruct (vector_inv_S rs) as (rsh & rst & hb).
-        destruct (vector_inv_S ms) as (msh & mst & hc).
-        destruct (vector_inv_S uscs) as (uscsh & uscst & hd).
-        destruct (vector_inv_S chs) as (chsh & chst & he).
-        subst. simpl. eapply Bool.andb_true_iff.
-        split.
-        ++
-          eapply vote_proof_valid.
-          exact (ha Fin.F1).
-        ++
-          eapply ihn.
-          intro f.
-          exact (ha (Fin.FS f)).
-    Qed.  
-  End Proofs.
+        assert (hb : sub u v = u + opp v). field.
+        rewrite hb in ha.
+        eapply f_equal with (f := fun x => x + v) in ha.
+        assert (hc : opp v + v = zero). field.
+        rewrite <-associative in ha.
+        rewrite hc in ha; clear hc.
+        assert (hc : u + zero = u) by field.
+        rewrite hc in ha; clear hc.
+        assert (hc : zero + v = v) by field.
+        rewrite hc in ha. exact ha.
+      Qed.
+        
+      
+      Theorem vote_proof_invalid_reject :
+        ∀ (r : F) (g h : G) (m : F)  (u₁ u₂ c₁ : F) (c : F),
+          g <> gid -> (m <> zero ∧ m <> one) → c₁ <> c ->
+          verify_encryption_vote_proof g h 
+            (encrypt_vote_and_generate_enc_proof r g h m [u₁; u₂; c₁] c) = false.
+      Proof.
+        intros * ht hu hv.
+        unfold encrypt_vote_and_generate_enc_proof, 
+        verify_encryption_vote_proof, generate_enc_proof.
+        destruct (Fdec m zero) as [fa | fa].
+        +
+          
+          destruct hu as (hal & har).
+          subst. specialize (hal eq_refl).
+          inversion hal.
+        +
+          destruct (Fdec m one) as [faa | faa].
+          ++
+            subst; destruct hu as (hal & har).
+            specialize (har eq_refl). 
+            inversion har.
+          ++
+            (* challenging case *)
+            unfold generalised_accepting_encryption_proof_elgamal, 
+            enc, generalised_construct_encryption_proof_elgamal_real, 
+            generate_enc_proof.
+            simpl. 
+            destruct (vector_fin_app_pred 1 (FS F1) [u₁; u₂] [c₁]) as
+            (m₁ & m₂ & v₁ & v₃ & vm & v₂ & v₄ & pfaa & pfbb & haa).
+            destruct pfaa as [pfa].
+            destruct pfbb as [pfb].
+            destruct haa as [ha].
+            destruct ha as (ha & hb & hc & hd).
+            subst; cbn in * |- *.
+            assert (m₂ = 0). 
+            {
+              destruct m₂ as [|m₂].
+              reflexivity. nia.
+            }
+            subst. cbn. 
+            assert (pfa = eq_refl). 
+            eapply Eqdep_dec.UIP_refl_nat.
+            assert (pfb = eq_refl). 
+            eapply Eqdep_dec.UIP_refl_nat.
+            subst. cbn in * |- *.
+            pose proof (vector_inv_0 v₂) as hd.
+            pose proof (vector_inv_0 v₄) as he.
+            rewrite hd, he in * |- *. cbn.
+            subst; cbn.
+            destruct (vector_inv_S v₁) as (ma & msr & hmm).
+            rewrite hmm in * |- *.
+            subst; cbn.
+            pose proof (vector_inv_0 msr) as hd.
+            subst; cbn.
+            destruct (vector_inv_S v₃) as (mb & msr & hmm).
+            subst; cbn.
+            pose proof (vector_inv_0 msr) as hd.
+            subst; cbn.
+            assert (hd : c = (c₁ + (sub c (c₁ + zero) + zero))). field.
+            rewrite <-hd; clear hd.
+            destruct (Fdec c c)
+            as [hdec | hdec]; try auto. 
+            eapply Bool.andb_false_intro2.
+            eapply Bool.andb_false_intro1.
+            eapply Bool.andb_false_intro2.
+            eapply dec_false; intro haa.
+            assert (hb : c₁ + zero = c₁). field.
+            rewrite !hb in haa; clear hb.
+            assert(hb : g ^ one = g).
+            rewrite field_one; reflexivity.
+            rewrite !hb in haa; clear hb.
+            assert (hb : gop (g ^ m) (h ^ r) = gop (h ^ r) (g ^ m)).
+            rewrite commutative. reflexivity.
+            rewrite !hb in haa; clear hb.
+            assert (hb : (gop (gop (h ^ r) (g ^ m)) (ginv g)) = 
+            gop (h ^ r) (gop (g ^ m) (ginv g))).
+            rewrite associative; reflexivity.
+            rewrite !hb in haa; clear hb.
+            remember ((gop (g ^ m) (ginv g))) as gp.
+            rewrite smul_distributive_vadd, smul_pow_mul,
+            associative in haa.
+            assert (hb : (gop (h ^ u₂) (h ^ (sub c c₁ * r))) = 
+              h ^ (u₂ + sub c c₁ * r)).
+            destruct Hvec. (* why do I need this destruct this? *)
+            setoid_rewrite <-vector_space_smul_distributive_fadd;
+            reflexivity.
+            rewrite hb in haa; clear hb.
+            eapply f_equal with (f := fun x => 
+              gop (h ^ (opp (u₂ + sub c c₁ * r))) x) in haa.
+            assert (hb : gop (h ^ opp (u₂ + sub c c₁ * r)) (h ^ (u₂ + sub c c₁ * r)) = gid).
+            destruct Hvec.
+            setoid_rewrite <-vector_space_smul_distributive_fadd.
+            assert (hb : (opp (u₂ + sub c c₁ * r) + (u₂ + sub c c₁ * r)) = zero). field.
+            rewrite hb; clear hb.
+            rewrite field_zero; reflexivity.
+            rewrite !hb in haa; clear hb.
+            rewrite associative in haa.
+            assert (hb : gop (h ^ opp (u₂ + sub c c₁ * r)) (h ^ (u₂ + sub c c₁ * r)) = 
+            gid). destruct Hvec.
+            rewrite <-vector_space_smul_distributive_fadd.
+            assert (hb : (opp (u₂ + sub c c₁ * r) + (u₂ + sub c c₁ * r)) = zero).
+            field. rewrite hb; clear hb.
+            rewrite field_zero; reflexivity.
+            rewrite hb in haa; clear hb.
+            rewrite left_identity in haa.
+            rewrite Heqgp in haa; clear Heqgp.
+            rewrite <- (vector_space_field_zero g) in haa.
+            assert (hb : gop (g ^ m) (ginv g) ^ sub c c₁ = 
+              gop ((g ^ m) ^ sub c c₁) (ginv g ^ sub c c₁)).
+            destruct Hvec.
+            rewrite vector_space_smul_distributive_vadd; reflexivity.
+            rewrite hb in haa; clear hb.
+            eapply f_equal with (f := fun x => gop x (g ^ sub c c₁)) in haa.
+            rewrite <-associative in haa.
+            assert (hb : (gop (ginv g ^ sub c c₁) (g ^ sub c c₁)) = gid).
+            destruct Hvec.
+            rewrite <-vector_space_smul_distributive_vadd, left_inverse, 
+            <-field_zero, smul_pow_up.
+            assert (hb : zero * sub c c₁ = zero). field.
+            rewrite hb; clear hb.
+            reflexivity.
+            rewrite hb in haa; clear hb.
+            destruct Hvec.
+            rewrite <- vector_space_smul_distributive_fadd, right_identity,
+            smul_pow_up in haa.
+            assert (hb : zero + sub c c₁ = sub c c₁). field.
+            rewrite hb in haa; clear hb.
+            eapply f_equal with (f := fun x => gop x (g ^ opp (sub c c₁))) in haa.
+            assert(hb : gop (g ^ sub c c₁) (g ^ opp (sub c c₁)) = gid).
+            destruct Hvec.
+            rewrite <-vector_space_smul_distributive_fadd.
+            assert(hb : (sub c c₁ + opp (sub c c₁)) = zero). field.
+            rewrite hb; clear hb.
+            rewrite field_zero; reflexivity.
+            rewrite !hb in haa; clear hb.
+            rewrite  <-smul_distributive_fadd in haa.
+            assert (hb : (m * sub c c₁ + opp (sub c c₁)) = 
+              (sub m one) * sub c c₁). field.
+            rewrite hb in haa; clear hb.
+            eapply eq_sym in haa.
+            eapply gid_power_zero in haa.
+            destruct haa as [haa | haa]; try congruence.
+            eapply mul_eq_zero in haa.
+            destruct haa as [haa | haa].
+            +++
+              eapply faa.
+              eapply sub_eq;
+              assumption.
+            +++
+              eapply hv.
+              eapply eq_sym.
+              eapply sub_eq.
+              assumption.
+          Unshelve.
+          exact g. exact Fdec.
+      Qed.
+
+
+      (* 
+        A theorem that states that if the prover can predict the challenge of 
+        the verifier, then it can fake the proof. 
+
+
+        if it is the case c = c₁ then 
+        an invalid proof will also be accepted but 
+        c = c₁ will happen with 1/|C| probability.
+      *)
+      Theorem vote_proof_invalid_accept :
+        ∀ (r : F) (g h : G) (m : F)  (u₁ u₂ c₁ : F) (c : F),
+          (m <> zero ∧ m <> one) → c₁ = c ->
+          verify_encryption_vote_proof g h 
+            (encrypt_vote_and_generate_enc_proof r g h m [u₁; u₂; c₁] c) = true.
+      Proof.
+        intros * [hal har] hb.
+        unfold encrypt_vote_and_generate_enc_proof, 
+        verify_encryption_vote_proof, 
+        generate_enc_proof.
+        eapply generalised_accepting_elgamal_conversations_correctness_gen.
+        destruct (Fdec m zero) as [fa | fa]; try congruence.
+        subst.
+        unfold generalised_accepting_encryption_proof_elgamal, 
+        enc, generalised_construct_encryption_proof_elgamal_real.
+        simpl. 
+        destruct (vector_fin_app_pred 1 (FS F1) [u₁; u₂] [c]) as
+          (m₁ & m₂ & v₁ & v₃ & vm & v₂ & v₄ & pfaa & pfbb & haa).
+        destruct pfaa as [pfa].
+        destruct pfbb as [pfb].
+        destruct haa as [ha].
+        destruct ha as (ha & hb & hc & hd).
+        subst; cbn in * |- *.
+        assert (m₂ = 0). 
+        {
+          destruct m₂ as [|m₂].
+          reflexivity. nia.
+        }
+        subst. cbn. 
+        assert (pfa = eq_refl). 
+        eapply Eqdep_dec.UIP_refl_nat.
+        assert (pfb = eq_refl). 
+        eapply Eqdep_dec.UIP_refl_nat.
+        subst. cbn in * |- *.
+        pose proof (vector_inv_0 v₂) as hd.
+        pose proof (vector_inv_0 v₄) as he.
+        rewrite hd, he in * |- *. cbn.
+        subst; cbn.
+        destruct (vector_inv_S v₁) as (ma & msr & hmm).
+        rewrite hmm in * |- *.
+        subst; cbn.
+        pose proof (vector_inv_0 msr) as hd.
+        subst; cbn.
+        destruct (vector_inv_S v₃) as (mb & msr & hmm).
+        subst; cbn.
+        pose proof (vector_inv_0 msr) as hd.
+        subst; cbn.
+        assert (hd : c = (c + (sub c (c + zero) + zero))). field.
+        rewrite <-hd; clear hd.
+        split. reflexivity.
+        intros f. rewrite !dec_true.
+        destruct (fin_inv_S _ f) as [f' | (f' & hf)].
+        +
+          subst; cbn.
+          split.
+          ++
+            pose proof @simulator_completeness F zero one add mul sub div opp inv 
+              G gid ginv gop gpow Gdec Hvec g (g ^ r) u₁ c as hb.
+            unfold accepting_conversation, schnorr_simulator in hb.
+            rewrite dec_true in hb; cbn in hb.
+            exact hb.
+          ++
+            assert(hb :  (ginv (g ^ zero)) = gid). 
+            rewrite field_zero, group_inv_id;
+            reflexivity.
+            rewrite !hb; clear hb.
+            remember (gop (g ^ m) (h ^ r)) as gm.
+            rewrite <-associative.
+            assert (hb : gop (gop gm gid ^ opp c) (gop gm gid ^ c) = gid). 
+            destruct Hvec.
+            rewrite <-vector_space_smul_distributive_fadd.
+            assert (hb : (opp c + c) = zero).
+            field. rewrite hb; clear hb.
+            rewrite field_zero; reflexivity.
+            rewrite hb; clear hb.
+            rewrite right_identity. 
+            reflexivity.
+        +
+          subst; cbn.
+          destruct (fin_inv_S _ f') as [f'' | (f'' & hf)];
+          subst; cbn; (try refine match f'' with end).
+          split.
+          ++
+            assert (hb : sub c (c + zero) * r = zero). field.
+            rewrite !hb; clear hb.
+            assert(hb : sub c (c + zero) = zero). field.
+            rewrite hb; clear hb.
+            rewrite field_zero, right_identity.
+            rewrite right_identity; reflexivity.
+          ++
+            assert (hb : sub c (c + zero) * r = zero). field.
+            rewrite !hb; clear hb.
+            assert(hb : sub c (c + zero) = zero). field.
+            rewrite hb; clear hb.
+            rewrite field_one, field_zero, 
+            right_identity, right_identity.
+            reflexivity.
+      Qed.
+
+
+      (* ballot proof is valid *)
+      Theorem ballot_proof_valid :
+        ∀ (n : nat) (rs : Vector.t F n) (g h : G) 
+          (ms : Vector.t F n) (uscs : Vector.t (Vector.t F 3) n) (chs : Vector.t F n),
+          (∀ (i : Fin.t n), Vector.nth ms i = zero ∨ Vector.nth ms i = one) ->
+          verify_encryption_ballot_proof g h 
+            (encrypt_ballot_and_generate_enc_proof rs g h ms uscs chs) = true.
+      Proof.
+        induction n as [|n ihn].
+        +
+          intros * ha.
+          pose proof (vector_inv_0 rs) as hb.
+          pose proof (vector_inv_0 ms) as hc.
+          pose proof (vector_inv_0 uscs) as hd.
+          pose proof (vector_inv_0 chs) as he.
+          subst; cbn. reflexivity.
+        +
+          intros * ha.
+          destruct (vector_inv_S rs) as (rsh & rst & hb).
+          destruct (vector_inv_S ms) as (msh & mst & hc).
+          destruct (vector_inv_S uscs) as (uscsh & uscst & hd).
+          destruct (vector_inv_S chs) as (chsh & chst & he).
+          subst. simpl. eapply Bool.andb_true_iff.
+          split.
+          ++
+            eapply vote_proof_valid.
+            exact (ha Fin.F1).
+          ++
+            eapply ihn.
+            intro f.
+            exact (ha (Fin.FS f)).
+      Qed.  
+    End Proofs.
 End Approval.
